SystemFD/Term/Substitution.lean
@@ -53,10 +53,13 @@ namespace Term
 
   -- k1 `-k> k2 `-k> k3 -→ [k1, k2, k3]
   @[simp]
-  def split_kind_arrow : List Term -> Term -> Option (List Term × Term)
-  | Γ, .ctor2 .arrowk f a => split_kind_arrow (f :: Γ) a
+  def split_kind_arrow_aux : List Term -> Term -> Option (List Term × Term)
+  | Γ, .ctor2 .arrowk f a => split_kind_arrow_aux (f :: Γ) a
   | Γ, ★ => .some (Γ, ★)
   | _, _ => .none
+
+  @[simp]
+  def split_kind_arrow : Term -> Option (List Term × Term) := split_kind_arrow_aux []
 
   @[simp]
   def mk_kind_app : Nat -> List Term -> Term := λ h sp =>
